Dafny/examples/Challenge8/Challenge8Benign.i.dfy
@@ -1,0 +1,21 @@
+include "Challenge8Code.s.dfy"
+include "../../LLVM/llvmREFACTOR_Multi.i.dfy"
+include "../../LLVM/types.dfy"
+
+
+module challenge8Benign{
+    import opened challenge8Code
+    import opened LLVM_defRE_Multi
+    import opened types
+
+
+    lemma equalBlocksEvalEqually(blockA:codeRe,blockB:codeRe)
+        requires blockA == blockB
+        ensures forall s :: ValidState(s) ==> evalCodeRE(blockA,s) == evalCodeRE(blockB,s);
+    {
+        assert forall s :: ValidState(s) ==> evalCodeRE(blockA,s) == evalCodeRE(blockB,s);
+    }
+
+
+}
+
